split yesno proofs into multiple files, working on mu-based no proof

fairis/heap_lang/examples/mu_role.v
@@ -29,26 +29,28 @@ Section MuRole.
     by iApply "MU".
   Qed.
 
-  (* Definition MU__drop ρ E P: iProp Σ :=   *)
-  (*   ∀ τ f R, τ ↦M ({[ ρ := f ]} ∪ (S <$> R)) ∗ ⌜ ρ ∉ dom R ⌝ -∗ *)
-  (*             MU E τ (τ ↦M R ∗ P) (LM := LM). *)
+  Definition MU__drop ρ E P: iProp Σ :=  
+    ∀ τ f R, τ ↦M ({[ ρ := f ]} ∪ R) ∗ ⌜ ρ ∉ dom R ⌝ -∗
+              (* MU E τ (τ ↦M R ∗ P) (LM := LM). *)
+               |~{ E }~| (τ ↦M R ∗ P).
 
-  (* Lemma MU__r_wand E ρ (P Q: iProp Σ): *)
-  (*   (P -∗ Q) -∗ MU__r ρ E P -∗ MU__r ρ E Q. *)
-  (* Proof. *)
-  (*   iIntros "HPQ HMU". rewrite /MU__r. iIntros "**". *)
-  (*   iSpecialize ("HMU" with "[$]").  *)
-  (*   iApply (MU_wand with "[HPQ] [$]"). iFrame. *)
-  (*   iIntros "[??]". iFrame. by iApply "HPQ".  *)
-  (* Qed. *)
+  Lemma MU__drop_mask_weaken E1 E2 ρ (P: iProp Σ)
+    (SUB: E1 ⊆ E2):
+    MU__drop ρ E1 P -∗ MU__drop ρ E2 P.
+  Proof.
+    iIntros "MU". rewrite /MU__drop. iIntros "**".
+    iMod pre_step_mask_subseteq as "CLOS"; [by apply SUB| ].
+    iMod ("MU" with "[$]") as "X". iMod "CLOS".
+    iModIntro. done. 
+  Qed.
 
-  (* Lemma MU__r_mask_weaken E1 E2 ρ (P: iProp Σ) *)
-  (*   (SUB: E1 ⊆ E2): *)
-  (*   MU__r ρ E1 P -∗ MU__r ρ E2 P. *)
-  (* Proof. *)
-  (*   iIntros "MU". rewrite /MU__r. iIntros "**". *)
-  (*   iApply MU_mask_weaken; eauto. *)
-  (*   by iApply "MU". *)
-  (* Qed. *)
+  Lemma MU__drop_wand E ρ (P Q: iProp Σ):
+    (P -∗ Q) -∗ MU__drop ρ E P -∗ MU__drop ρ E Q.
+  Proof.
+    iIntros "PQ MU". rewrite /MU__drop. iIntros "**".
+    iSpecialize ("MU" with "[$]"). 
+    iApply (pre_step_mono with "[PQ] [$]").
+    iIntros "[??]". iFrame. by iApply "PQ". 
+  Qed.
 
 End MuRole.
