fairis/heap_lang/examples/yesno/yesno.v
@@ -7,15 +7,13 @@ From iris.proofmode Require Import tactics.
 From trillium.prelude Require Export finitary quantifiers sigma classical_instances.
 From trillium.program_logic Require Export weakestpre.
 From trillium.fairness Require Import fairness fair_termination fuel sswp_rules resources action_model utils.
-From trillium.fairness.heap_lang Require Export lang lifting tactics proofmode  notation iris_inst.
-From trillium.fairness.heap_lang.examples Require Import env_am split_model.
-From trillium.fairness.heap_lang.examples Require Import mu_role.
+From trillium.fairness.heap_lang Require Export lang lifting tactics proofmode notation iris_inst.
+From trillium.fairness.heap_lang.examples Require Import env_am split_model mu_role.
+From trillium.fairness.heap_lang.examples.yesno Require Import yesno_model yesno_mus.
 
 Import derived_laws_later.bi.
 
 Open Scope nat.
-
-Set Default Proof Using "Type".
 
 Definition go_impl (b: bool): val :=
   rec: "go_impl" "n" "b" :=
@@ -35,169 +33,9 @@ Definition no : val :=
 Definition start : val :=
   λ: "N", let: "b" := Alloc #true in (Fork (yes "N" "b") ;; Fork (no "N" "b")).
 
-(** * Definition of the model! *)
-
-Inductive YN := Y | No.
-
-#[global] Instance YN_eqdec: EqDecision YN.
-Proof. solve_decision. Qed.
-
-#[global] Instance YN_countable: Countable YN.
-Proof.
-  refine ({|
-             encode yn := match yn with Y => 1 | No => 2 end;
-             decode p := match p with 1 => Some Y | 2 => Some No | _ => None end;
-         |})%positive.
-  intros yn. by destruct yn.
-Qed.
-
-#[global] Instance YN_inhabited: Inhabited YN.
-Proof. exact (populate Y). Qed.
-
-Definition yn_act: Action := coPpick (↑ nroot .@ "yesno"). 
-
-Inductive yntrans: nat*bool -> (Action * option YN) -> nat*bool -> Prop :=
-| yes_trans n: (n > 0)%nat -> yntrans (n, true) (yn_act, Some Y) (n, false) (* < *)
-| yes_fail n: (n > 1)%nat -> yntrans (n, false) (yn_act, Some Y) (n, false) (* ≤ *)
-| no_trans n: yntrans (S n, false) (yn_act, Some No) (n, true) (* < *)
-| no_fail n: (n > 0)%nat → yntrans (n, true) (yn_act, Some No) (n, true) (* ≤ *)
-.
-
-Definition yn_live_roles nb : gset YN :=
-  match nb with
-  | (0, _) => ∅
-  | (1, false) => {[ No ]}
-  | _ => {[ No; Y ]}
-  end.
-
-Definition yn_AM: ActionModel := {| amTrans := yntrans |}.
-
-Instance yn_step_dec: AM_step_dec yn_AM. 
-Proof. 
-  red. intros [n1 b1] a oρ [n2 b2].
-  Local Ltac nostep := right; intros STEP; inversion STEP; try (subst; tauto || lia). 
-  destruct (decide (a = yn_act)) as [-> | ].
-  2: { by nostep. }
-  destruct oρ as [ρ| ]; [| by nostep].
-  destruct (decide (n2 = n1 /\ b1 = true /\ b2 = false /\ ρ = Y /\ 0 < n1)) as [S| ]. 
-  { destruct S as (->&->&->&->&?).
-    left. simpl. by constructor. } 
-  destruct (decide (n2 = n1 /\ b1 = false /\ b2 = false /\ ρ = Y /\ 1 < n1)) as [S| ]. 
-  { destruct S as (->&->&->&->&?).
-    left. simpl. by constructor. } 
-  destruct (decide (n1 = S n2 /\ b1 = false /\ b2 = true /\ ρ = No)) as [S| ]. 
-  { destruct S as (->&->&->&->).
-    left. simpl. by constructor. } 
-  destruct (decide (n2 = n1 /\ b1 = true /\ b2 = true /\ ρ = No /\ 0 < n1)) as [S| ]. 
-  { destruct S as (->&->&->&->&?).
-    left. simpl. by constructor. }
-  by nostep.
-Qed. 
-
-Instance yn_fb: AM_fin_branch' yn_AM.
-Proof.
-  exists (fun '(n, b) => 
-         n' ← [n; (n-1)%nat];
-         w' ← [b; negb b];
-         ℓ ← [Some Y; Some No];
-         mret ((n', w'), yn_act, ℓ)). 
-  intros [??] [??] ?? Htrans.
-  repeat setoid_rewrite elem_of_list_bind.
-  setoid_rewrite elem_of_list_ret.
-  setoid_rewrite (and_comm (exists _, _) _).
-  setoid_rewrite <- utils.ex_and_comm. rewrite utils.ex_prod'.
-  setoid_rewrite (and_comm _ (_ /\ _)).
-  setoid_rewrite <- (and_assoc _ _). 
-  setoid_rewrite (and_comm _ (_ /\ _)).
-  setoid_rewrite <- utils.ex_and_comm. rewrite utils.ex_prod'.
-  eapply utils.ex_det_iff.
-  { intros [[? ?] ?] (?&EQ&?). simpl in EQ.
-    inversion EQ. subst. reflexivity. }
-  simpl.
-  inversion Htrans; subst; simpl; try set_solver.
-  repeat split; try set_solver.
-  rewrite Nat.sub_0_r. set_solver.
-Qed. 
-
-Lemma yn_AM_live_roles (nb: amSt yn_AM) ρ:
-  ρ ∈ AM_live_roles nb <-> ρ ∈ yn_live_roles nb.
-Proof.
-  destruct nb as [n b]. 
-  rewrite -AM_live_roles_spec. simpl.
-  destruct n as [| [| ]], b; simpl.
-  - split; [| done]. intros (?&?&STEP). inversion STEP; lia.
-  - split; [| done]. intros (?&?&STEP). inversion STEP; lia.
-  - split.
-    + intros (?&?&STEP). inversion STEP; set_solver.
-    + rewrite elem_of_union !elem_of_singleton. intros [-> | ->].
-      all: do 2 eexists; constructor; lia.  
-  - rewrite !elem_of_singleton. 
-    split.
-    + intros (?&?&STEP). inversion STEP; try lia || done.
-    + intros ->. do 2 eexists. constructor.
-  - split.
-    + intros (?&?&STEP). inversion STEP; set_solver.
-    + rewrite elem_of_union !elem_of_singleton. intros [-> | ->].
-      all: do 2 eexists; constructor; lia.  
-  - split.
-    + intros (?&?&STEP). inversion STEP; set_solver.
-    + rewrite elem_of_union !elem_of_singleton. intros [-> | ->].
-      all: do 2 eexists; constructor; lia.  
-Qed.
-
-Lemma yn_acts: forall a, is_action_of yn_AM a <-> a = yn_act.
-Proof. 
-  intros. rewrite /is_action_of. split.
-  - intros (?&?&?&STEP). inversion STEP; eauto.
-  - intros ->.
-    do 3 eexists. econstructor. eauto.
-Qed. 
-
-Lemma yn_AM_live_roles' (st: amSt yn_AM):
-  AM_live_roles st = yn_live_roles st.
-Proof. 
-  apply set_eq. intros. rewrite -yn_AM_live_roles. done.
-Qed. 
-
-Instance yn_AM_act_dec: forall a, Decision (is_action_of yn_AM a).
-Proof.
-  intros. eapply Decision_iff_impl; [symmetry; apply yn_acts| ].
-  apply _.
-Qed. 
   
-(** The CMRAs we need. *)
-Class yesnoG Σ := YesnoG {
-  yes_name: gname;
-  no_name: gname;
-  yesno_n_G :> inG Σ (excl_authR natO);
-  yesno_f_G :> inG Σ (excl_authR boolO);
- }.
-Class yesnoPreG Σ := {
-  yesno_PreG :> inG Σ (excl_authR natO);
-  yesno_f_PreG :> inG Σ (excl_authR boolO);
- }.
-
-
-Section FullModel.
-  Context `(ENV_AM: EnvironmentAM env_AM).
-
-  Definition FM := ProdAM env_AM yn_AM.
-  
-  Definition the_fair_model: FairModel := AM2FM FM _. 
-  
-  Definition the_model: LiveModel heap_lang the_fair_model :=
-    {| lm_flm := 61%nat; |}.
-  
-  Definition yesnoΣ : gFunctors :=
-    #[ heapΣ the_fair_model; GFunctor (excl_authR natO) ; GFunctor (excl_authR boolO) ].
-
-  Global Instance subG_yesnoΣ {Σ} : subG yesnoΣ Σ → yesnoPreG Σ.
-  Proof. solve_inG. Qed.
-
-End FullModel.
-
-
 Section proof.
+  
   Context `(ENV_AM: EnvironmentAM env_AM).
   Context {INDEP: models_independent env_AM yn_AM}.
 
@@ -207,329 +45,16 @@ Section proof.
 
   Context `{!heapGS Σ LM, !yesnoG Σ, SplitGS Σ env_AM yn_AM}.
 
-  Let Ns := nroot .@ "yes_no".
-
-  Definition yes_at (n: nat) := own yes_name (◯E n).
-  Definition no_at (n: nat) := own no_name (◯E n).
-
-  Definition auth_yes_at (n: nat) := own yes_name (●E n).
-  Definition auth_no_at (n: nat) := own no_name (●E n).
-
-  Lemma they_agree γ (n m: nat) :
-    own γ (◯E n) -∗ own γ (●E m) -∗ ⌜ m = n ⌝.
-  Proof.
-    iIntros "HA HB". iCombine "HB HA" as "H".
-    iDestruct (own_valid with "H") as "%Hval".
-    iPureIntro. by apply excl_auth_agree_L.
-  Qed.
-  Lemma yes_agree n m :
-    yes_at n -∗ auth_yes_at m -∗ ⌜ m = n ⌝.
-  Proof. apply they_agree. Qed.
-  Lemma no_agree n m :
-    no_at n -∗ auth_no_at m -∗ ⌜ m = n ⌝.
-  Proof. apply they_agree. Qed.
-
-  Lemma they_update γ (n m P: nat) :
-    own γ (●E n) ∗ own γ (◯E m) ==∗ own γ (●E P) ∗ own γ (◯E P).
-  Proof.
-    rewrite -!own_op. iApply own_update. apply excl_auth_update.
-  Qed.
-  Lemma yes_update P n m :
-     auth_yes_at m ∗ yes_at n ==∗ auth_yes_at P ∗ yes_at P.
-  Proof. apply they_update. Qed.
-  Lemma no_update P n m :
-     auth_no_at m ∗ no_at n ==∗ auth_no_at P ∗ no_at P.
-  Proof. apply they_update. Qed.
-
-  Lemma they_finished_update γ (n m P: bool) :
-    own γ (●E n) ∗ own γ (◯E m) ==∗ own γ (●E P) ∗ own γ (◯E P).
-  Proof.
-    rewrite -!own_op. iApply own_update. apply excl_auth_update.
-  Qed.
-
-  Definition yn_corr l n b: iProp Σ := 
-      (⌜(n, b) ≠ (0, false)⌝ ∗
-      (* frag_right_st_is (n, b) ∗ *)
-      l ↦ #b ∗
-      if b
-      then auth_yes_at n ∗ auth_no_at n
-      else auth_yes_at (n-1) ∗ auth_no_at n)%I.
-
-  Definition yesno_inv_inner b : iProp Σ :=
-    ∃ n B,
-      yn_corr b n B ∗
-      frag_right_st_is (n, B). 
-
-  Definition yesno_inv b := inv Ns (yesno_inv_inner b).
-
-  Definition Ns__split := nroot .@ "split".
-
   Let yn_role (ρ: YN): amRole PM := inr ρ.
 
-  Lemma yes_go_spec tid n b (N: nat) f (Hf: f > 40):
-    {{{ split_inv Ns__split ∗ yesno_inv b ∗ tid ↦M {[ yn_role Y := f ]} ∗ n ↦ #N ∗ ⌜N > 0⌝%nat ∗
-        yes_at N }}}
-      yes_go #n #b @ tid
-    {{{ RET #(); tid ↦M ∅ }}}.
-  Proof using INDEP.
-    iLöb as "Hg" forall (N f Hf).
-    iIntros (Φ) "(#SPLIT & #Hinv & Hf & HnN & %HN & Hyes) Hk". unfold yes_go, go_impl.
-    wp_pures.
-    wp_bind (CmpXchg _ _ _).
-    iApply wp_atomic.
-    iInv Ns as (m B) "((>%Hnever & >Bb & Hauths) & >Hmod)" "Hclose".
-    iInv Ns__split as ([e ?]) "(>ST & >PROD)" "Hclose'".
-    simpl. 
-    iDestruct (right_agree with "PROD Hmod") as %->.
-
-    rewrite if_arg2_comm. iDestruct "Hauths" as "[Hay Han]". 
-    rewrite !if_arg_comm. iMod "Hay". iMod "Han".
-    iDestruct (yes_agree with "Hyes Hay") as %Heq.
-    
-    assert (amTrans yn_AM (m, B) (yn_act, Some Y) (m, false)) as STEP.
-    { destruct B; econstructor; lia. }
-
-    destruct B. 
-    - destruct (decide (m= 0)) as [->|Nneq]; first lia.
-      iModIntro.
-      subst N.
-
-      iApply sswp_MU_wp; [done| ].
-      iApply (wp_cmpxchg_suc with "[$]"); try done.
-      iIntros "!> Hb". 
-
-      iApply (MU_wand with "[-ST Hf]").
-      2: { iApply (model_step_singlerole_MU with "[$] [$]"). 
-           { simpl. do 2 econstructor; eauto.
-             intros ?. apply action_of_step in STEP.
-             edestruct INDEP; eauto. }
-           simpl. rewrite !(prod_indep_live_roles _ _ INDEP). 
-           rewrite !yn_AM_live_roles'. simpl.
-           apply union_mono; [done| ].
-           destruct m as [|[|]]; [lia| ..]; set_solver. }
-      iIntros "[ST Hf]".
-
-      iMod (yes_update (m - 1) with "[$]") as "[Hay Hyes]".
-      iMod (update_right ((m, false): amSt yn_AM) with "[$] [$]") as "[PROD Hmod]".
-      wp_pures.
-      iModIntro. 
-      iMod ("Hclose'" with "[PROD ST]") as "_".
-      { iFrame. }
-      iMod ("Hclose" with "[Hmod Hb Hay Han]") as "_".
-      { iNext. iExists _, _. iFrame. simpl. iFrame.
-        iPureIntro. by intros [=]. }
-      iModIntro. 
-      
-      simpl in *. wp_load. wp_store. wp_load. wp_pure _.
-      destruct m; [lia| ].
-      destruct m. 
-      + rewrite bool_decide_eq_false_2.
-        2: { lia. }
-        iApply wp_atomic.
-        iInv Ns as (m B) "((>%Hbever' & >Hb & Hauths) & >Hmod)" "Hclose".
-        clear e. iInv Ns__split as ([e ?]) "(>ST & >PROD)" "Hclose_".
-        iDestruct (right_agree with "PROD Hmod") as %EQ. simpl in EQ. subst. simpl.
-        rewrite if_arg2_comm. iDestruct "Hauths" as "[Hay Han]". 
-        rewrite !if_arg_comm. iMod "Hay". iMod "Han".
-        iDestruct (yes_agree with "Hyes Hay") as %Heq.
-        
-        iAssert (⌜ m= 0 /\ B = true \/ m= 1 /\ B = false ⌝)%I as %EQ.
-        { iPureIntro. destruct B; [tauto| ]. 
-          right. split; [| done].
-          destruct m as [|[|]]; try lia. done. }
-        iModIntro.
-
-        iApply wp_pre_step. wp_pure _. 
-        iApply fupd_mask_intro; [done|].
-        iIntros "Hclose'".
-        rewrite insert_empty.
-        iMod (has_fuels_dealloc _ _ _ (yn_role Y: fmrole M) with "ST Hf") as "[ST Hf]".
-        { simpl. rewrite prod_indep_live_roles. apply not_elem_of_union.
-          split; [set_solver| ]. 
-          intros IN%elem_of_map_inj_gset; [| by apply _]. 
-          rewrite yn_AM_live_roles in IN.
-          destruct EQ as [[-> ->]|[-> ->]]; set_solver. }
-        iModIntro.
-        iMod ("Hclose_" with "[PROD ST]").
-        { iFrame. }
-        iMod ("Hclose" with "[Hmod Hay Han Hb]").
-        { iNext. iExists _, _. iFrame.
-          destruct EQ as [[-> ->]|[-> ->]]; iFrame; done. }
-        iModIntro. iApply "Hk".
-        rewrite delete_insert; [|set_solver].
-        iFrame "Hf".
-      + rewrite bool_decide_eq_true_2 //; last lia.
-        wp_pure _.
-        iApply ("Hg" with "[] [Hyes HnN Hf] [$]"); last first.
-        { iFrame "∗#". iSplit; last by iPureIntro; lia.
-          by rewrite Nat2Z.inj_sub; [| lia]. }
-        iPureIntro; lia.
-    - have HM: m> 0 by lia.
-      iModIntro.
-
-      iApply sswp_MU_wp; [done| ].
-      iApply (wp_cmpxchg_fail with "[$]"); try done.
-      iIntros "!> Hb". 
-      iApply (MU_wand with "[-ST Hf]").
-      2: { iApply (model_step_singlerole_MU with "[$] [$]"). 
-           { simpl. do 2 econstructor; eauto.
-             intros ?. apply action_of_step in STEP. 
-             edestruct INDEP; eauto. }
-           set_solver. }
-      iIntros "[ST Hf]".
-      wp_pures. iModIntro.
-      iMod ("Hclose'" with "[ST PROD]").
-      { iFrame. simpl. iFrame. }
-      iMod ("Hclose" with "[Hmod Hb Hay Han]").
-      { iNext. simplify_eq. iExists _, _. iFrame. iFrame. done. }
-      iModIntro.
-      simpl. wp_load. wp_pure _. rewrite bool_decide_eq_true_2; last lia.
-      wp_pure _.
-      iApply ("Hg" with "[] [Hyes HnN Hf] [$]"); last first.
-      { iFrame "∗#". iPureIntro; lia. }
-      iPureIntro; lia.
-  (* This proof works but takes forever to typecheck *)
-  (* Time Qed. *)
-  Abort. 
-
-  Definition MU__drop ρ E P: iProp Σ :=  
-    ∀ τ f R, τ ↦M ({[ ρ := f ]} ∪ R) ∗ ⌜ ρ ∉ dom R ⌝ -∗
-              (* MU E τ (τ ↦M R ∗ P) (LM := LM). *)
-               |~{ E }~| (τ ↦M R ∗ P).
-
-  (* TODO: some of updates should drop the role *)
-  Definition yes_vs l ι: iProp Σ :=
-    □ |={⊤, ⊤ ∖ ↑ι}=> ∃ n b,
-      (▷ yn_corr l n b) ∗
-      ((⌜ if b then n > 0 else n > 1 ⌝ -∗ MU__r (yn_role Y) (⊤ ∖ ↑ι)
-         (* redundancy to ease subsequent adaptation for No thread *)
-           (▷ (if b then yn_corr l n false else yn_corr l n false) ={⊤ ∖ ↑ι, ⊤}=∗ True)
-       ) ∧
-       (⌜ n = 0 /\ b = true \/ n = 1 /\ b = false ⌝ -∗ 
-        MU__drop (yn_role Y) (⊤ ∖ ↑ι) (▷ yn_corr l n b ={⊤ ∖ ↑ι, ⊤}=∗ True))
-      ).
-
-  Lemma mu_yes n (b: bool) (ns: namespace)
-    (NB: if b then n > 0 else n > 1):
-    inv ns (split_inv_inner) ⊢ frag_right_st_is (n, b) -∗ 
-      MU__r (yn_role Y) (↑ ns) (frag_right_st_is $ if b then (n, false) else (n, false)).
-  Proof using INDEP.
-    rewrite /MU__r. iIntros "#INV ST" (tid f' R) "[MAP %DISJ__R]".
-    (* destruct st as [[st__e st__o] st__env]. *)
-
-    enough (exists a, amTrans yn_AM (n, b) (a, Some Y) (if b then (n, false) else (n, false))) as (a & TRANS). 
-    { iApply (MU_inv with "[$]"); [done| ].
-      (* TODO: avoid unfolding of MU *)
-      rewrite /split_inv_inner. simpl. iIntros ">(%S & FRAG & PROD)". destruct S.
-      simpl. iDestruct (right_agree with "[$] [$]") as %->.
-
-      iMod (update_right ((if b then (n, false) else (n, false)): amSt yn_AM) with "[$] [$]") as "[PROD ST]".
-      iApply (MU_wand with "[ST PROD]").
-      2: { iApply (model_step_MU with "[$] [MAP]").
-           1, 4: by eauto.
-           { simpl. eapply am_fmtrans_action. eexists. 
-             eapply pt_inner2; eauto.
-             intros ?. edestruct INDEP; eauto.
-             eapply action_of_step; eauto. }
-           simpl. setoid_rewrite @prod_indep_live_roles; eauto.
-           apply union_mono; [done| ]. apply set_map_mono; [done| ].
-           erewrite !yn_AM_live_roles'.
-           simpl. destruct b, n as [|[|]]; set_solver. }
-      iIntros "(MAP & FRAG)".
-      iFrame. }
-    Unshelve. 2: by apply _.
-
-    exists yn_act. simpl. destruct b; by constructor. 
-  Qed.
-
-  Lemma dealloc_yes n (b: bool) (ns: namespace)
-    (NB: n = 0 /\ b = true \/ n = 1 /\ b = false):
-    inv ns (split_inv_inner) ⊢ frag_right_st_is (n, b) -∗
-        MU__drop (yn_role Y) (↑ ns) (frag_right_st_is (n, b)). 
-  Proof using INDEP. 
-    rewrite /MU__drop. iIntros "#INV ST" (tid f' R) "[MAP %DISJ__R]".
-
-    iApply (pre_step_inv with "[$]"); [done| ].
-    rewrite /split_inv_inner. simpl. iIntros "(%S & FRAG & PROD)". destruct S.
-    iApply fupd_pre_step. iMod "FRAG". iMod "PROD". iModIntro. 
-    simpl. iDestruct (right_agree with "[$] [$]") as %->.
-
-    (* iApply (pre_step_mono with "[ST MAP]"). *)
-    (* 2: { iApply (has_fuels_dealloc with "[$]").  *)
-    
-    iMod (has_fuels_dealloc _ _ _ (yn_role Y: fmrole M) with "FRAG MAP") as "[FRAG MAP]".
-    { simpl. rewrite prod_indep_live_roles. apply not_elem_of_union.
-      split; [set_solver| ].
-      intros IN%elem_of_map_inj_gset; [| by apply _].
-      rewrite yn_AM_live_roles in IN.
-      destruct NB as [[-> ->]|[-> ->]]; set_solver. }
-
-    iModIntro. rewrite -insert_union_singleton_l delete_insert_dom.
-    2: set_solver.
-    by iFrame.
+  Lemma insert_empty_fmap_helper `{Countable K} {A: Type} (k: K) (a: A) (f: A -> A):
+    (<[ k := a ]> ∅: gmap K A) = {[ k := a ]} ∪ (f <$> ∅).
+  Proof.
+    rewrite insert_union_singleton_l. f_equiv. done.
   Qed. 
 
-  (* TODO: move *)
-  Lemma MU__drop_mask_weaken E1 E2 ρ (P: iProp Σ)
-    (SUB: E1 ⊆ E2):
-    MU__drop ρ E1 P -∗ MU__drop ρ E2 P.
-  Proof.
-    iIntros "MU". rewrite /MU__drop. iIntros "**".
-    iMod pre_step_mask_subseteq as "CLOS"; [by apply SUB| ].
-    iMod ("MU" with "[$]") as "X". iMod "CLOS".
-    iModIntro. done. 
-  Qed.
-
-  (* TODO: move *)
-  Lemma MU__drop_wand E ρ (P Q: iProp Σ):
-    (P -∗ Q) -∗ MU__drop ρ E P -∗ MU__drop ρ E Q.
-  Proof.
-    iIntros "PQ MU". rewrite /MU__drop. iIntros "**".
-    iSpecialize ("MU" with "[$]"). 
-    iApply (pre_step_mono with "[PQ] [$]").
-    iIntros "[??]". iFrame. by iApply "PQ". 
-  Qed.
-
-  Lemma yes_vs_from_invs l:
-    yesno_inv l ∗ split_inv Ns__split  ⊢ yes_vs l Ns.
-  Proof using INDEP.
-    rewrite /yes_vs. iIntros "#[INV1 INV2]". iModIntro.
-    iMod (inv_acc with "INV1") as "[OPEN CLOS]".
-    { apply top_subseteq. }
-    
-    rewrite {1}/yesno_inv_inner. rewrite {1}/yn_corr.  
-    iDestruct "OPEN" as (n b) "((>%NEQ & >LOC & AUTHS) & >RIGHT)".
-    iModIntro.
-    iExists _, _. iSplitL "LOC AUTHS".
-    { by iFrame. }
-
-    iSplit. 
-    - iIntros "%B". 
-      iApply (MU__r_mask_weaken (↑ Ns__split) with "[-]").
-      { assert (Ns__split ## Ns) by solve_ndisj. set_solver. }
-      iApply (MU__r_wand with "[-RIGHT]").
-      2: { by iApply (mu_yes with "[$] [$]"). }
-      iIntros "RIGHT CORR".
-      iMod ("CLOS" with "[-]"); [| done].
-      rewrite /yesno_inv_inner. iNext.
-      (* some redundancy to ease subsequent "No" proofs *)
-      iExists (if b then n else n), (if b then false else false).
-      destruct b; iFrame.
-    - iIntros "%NB". 
-      iApply (MU__drop_mask_weaken (↑ Ns__split) with "[-]").
-      { assert (Ns__split ## Ns) by solve_ndisj. set_solver. }
-      iApply (MU__drop_wand with "[-RIGHT]"). 
-      2: { by iApply (dealloc_yes with "[$]"). }
-      iIntros "RIGHT CORR".
-      iMod ("CLOS" with "[-]"); [| done].
-      rewrite /yesno_inv_inner. iNext.
-      iFrame. 
-  Qed.
-
-  Lemma yes_go_spec_vs tid n b (N: nat) f (Hf: f > 40):
-    {{{ (* split_inv Ns__split ∗ *)
-        (* yesno_inv b ∗ *)
-        yes_vs b Ns ∗
+  Lemma yes_go_spec_vs Ns tid n b (N: nat) f (Hf: f > 40):
+    {{{ yes_vs ENV_AM b Ns ∗
         tid ↦M {[ yn_role Y := f ]} ∗ n ↦ #N ∗ ⌜N > 0⌝%nat ∗
         yes_at N }}}
       yes_go #n #b @ tid
@@ -545,18 +70,12 @@ Section proof.
     iMod "V" as "(%m & %B & ((>%Hnever & >Bb & Hauths) & V))".
     iDestruct (bi.and_elim_l with "V") as "MU_y".       
 
-    (* iInv Ns__split as ([e ?]) "(>ST & >PROD)" "Hclose'". *)
     simpl. 
-
-    (* iDestruct (right_agree with "PROD Hmod") as %->. *)
 
     rewrite if_arg2_comm. iDestruct "Hauths" as "[Hay Han]". 
     rewrite !if_arg_comm. iMod "Hay". iMod "Han".
     iDestruct (yes_agree with "Hyes Hay") as %Heq.
     
-    (* assert (amTrans yn_AM (m, B) (yn_act, Some Y) (m, false)) as STEP. *)
-    (* { destruct B; econstructor; lia. } *)
-
     destruct B. 
     - destruct (decide (m= 0)) as [->|Nneq]; first lia.
       iModIntro.
@@ -570,11 +89,9 @@ Section proof.
       2: { iSpecialize ("MU_y" with "[] [Hf]").
            { iPureIntro. lia. }
            2: { by iFrame. }
-           iSplitL.
-           { iApply has_fuels_proper; [reflexivity| | by iFrame].
-             rewrite insert_union_singleton_l. f_equiv.
-             apply leibniz_equiv_iff, fmap_empty. }
-           iPureIntro. set_solver. } 
+           iSplitL. 
+           { erewrite insert_empty_fmap_helper. by iFrame. }
+           iPureIntro. set_solver. }
 
       iIntros "[Hf CLOS]".
 
@@ -601,7 +118,7 @@ Section proof.
         rewrite !if_arg_comm. iMod "Hay". iMod "Han".
         iDestruct (yes_agree with "Hyes Hay") as %Heq.
         
-        iAssert (⌜ m= 0 /\ B = true \/ m= 1 /\ B = false ⌝)%I as %EQ.
+        iAssert (⌜ m = 0 /\ B = true \/ m = 1 /\ B = false ⌝)%I as %EQ.
         { iPureIntro. destruct B; [tauto| ]. 
           right. split; [| done].
           destruct m as [|[|]]; try lia. done. }
@@ -610,13 +127,12 @@ Section proof.
         iApply wp_pre_step. wp_pure _. 
         iApply fupd_mask_intro; [done|].
         iIntros "Hclose'".
-        rewrite insert_empty.
 
         iSpecialize ("DEALLOC" with "[//] [Hf]").
         { iSplitL.
-          { iApply has_fuels_proper; [reflexivity| | by iFrame].
-            apply leibniz_equiv_iff, map_union_empty. }
-          iPureIntro. set_solver. }
+          { erewrite insert_empty_fmap_helper. by iFrame. }
+          iPureIntro. rewrite dom_fmap. set_solver. }
+        Unshelve. 2: exact id. 
  
         iApply (pre_step_mono with "[-DEALLOC] [$]").
         iIntros "[MAP CORR]".
@@ -642,9 +158,7 @@ Section proof.
            { iPureIntro. lia. }
            2: by iFrame.
            iSplitL.
-           { iApply has_fuels_proper; [reflexivity| | by iFrame].
-             rewrite insert_union_singleton_l. f_equiv.
-             apply leibniz_equiv_iff, fmap_empty. }
+           { erewrite insert_empty_fmap_helper; by iFrame. }
            iPureIntro. set_solver. }
 
       iIntros "[Hf CLOS]".
@@ -661,7 +175,7 @@ Section proof.
   Time Qed.
   
   Lemma yes_spec tid b (N: nat) f (Hf: f > 50):
-    {{{ split_inv Ns__split ∗ yesno_inv b ∗ tid ↦M {[ yn_role Y := f ]} ∗ ⌜N > 0⌝ ∗ yes_at N }}}
+    {{{ split_inv Ns__split ∗ yesno_inv ENV_AM b ∗ tid ↦M {[ yn_role Y := f ]} ∗ ⌜N > 0⌝ ∗ yes_at N }}}
       yes #N #b @ tid
     {{{ RET #(); tid ↦M ∅ }}}.
   Proof using INDEP.
@@ -680,12 +194,12 @@ Section proof.
   Qed.
 
   Lemma no_go_spec tid n b (N: nat) f (Hf: f > 40):
-    {{{ split_inv Ns__split ∗ yesno_inv b ∗ tid ↦M {[ yn_role No := f ]} ∗ n ↦ #N ∗ ⌜N > 0⌝ ∗ no_at N }}}
+    {{{ split_inv Ns__split ∗ yesno_inv ENV_AM b ∗ tid ↦M {[ yn_role No := f ]} ∗ n ↦ #N ∗ ⌜N > 0⌝ ∗ no_at N }}}
       no_go #n #b @ tid
     {{{ RET #(); tid ↦M ∅ }}}.
   Proof.
     (* iLöb as "Hg" forall (N f Hf). *)
-    (* iIntros (Φ) "(#Hinv & Hf & HnN & %HN & Hno) Hk". unfold no_go, go_impl. *)
+    (* iIntros (Φ) "(#SPLIT & #Hinv & Hf & HnN & %HN & Hno) Hk". unfold no_go, go_impl. *)
     (* wp_pures. *)
     (* wp_bind (CmpXchg _ _ _). *)
     (* assert (∀ s, Atomic s (CmpXchg #b #true #false)) by apply _. *)
@@ -771,24 +285,158 @@ Section proof.
     (*   iApply ("Hg" with "[] [Hno HnN Hf] [$]"); last first. *)
     (*   { iFrame "∗#". iPureIntro; lia. } *)
     (*   iPureIntro; lia. *)
-  Admitted. 
+  Admitted.
+
+
+  Definition no_vs l ι: iProp Σ :=
+    □ |={⊤, ⊤ ∖ ↑ι}=> ∃ n b,
+      (▷ yn_corr ENV_AM l n b) ∗
+      ((⌜ if b then n > 0 else n > 0 ⌝ -∗ MU__r (yn_role No) (⊤ ∖ ↑ι)
+           (▷ (if b then yn_corr ENV_AM l n true else yn_corr ENV_AM l (n - 1) true) ={⊤ ∖ ↑ι, ⊤}=∗ True)
+       ) ∧
+       (
+         (* ⌜ n = 0 /\ b = true \/ n = 1 /\ b = false ⌝ -∗  *)
+         ⌜ n = 0 ⌝ -∗
+        MU__drop (yn_role No) (⊤ ∖ ↑ι) (▷ yn_corr ENV_AM l n b ={⊤ ∖ ↑ι, ⊤}=∗ True))
+      ).
+
+  Lemma no_go_spec_vs Ns tid n b (N: nat) f (Hf: f > 40):
+    {{{ no_vs b Ns ∗
+        tid ↦M {[ yn_role No := f ]} ∗ n ↦ #N ∗ ⌜N > 0⌝%nat ∗
+        no_at N }}}
+      no_go #n #b @ tid
+    {{{ RET #(); tid ↦M ∅ }}}.
+  Proof using INDEP.
+    iLöb as "Hg" forall (N f Hf).
+    iIntros (Φ) "(#VS & Hf & HnN & %HN & HNo) Hk". unfold no_go, go_impl.
+    wp_pures.
+    wp_bind (CmpXchg _ _ _).
+    iApply wp_atomic.
+
+    iPoseProof "VS" as "-#V". 
+    iMod "V" as "(%m & %B & ((>%Hnever & >Bb & Hauths) & V))".
+    iDestruct (bi.and_elim_l with "V") as "MU_no".
+
+    simpl. 
+
+    rewrite if_arg2_comm. iDestruct "Hauths" as "[Hay Han]". 
+    rewrite !if_arg_comm. iMod "Hay". iMod "Han".
+    iDestruct (no_agree with "HNo Han") as %Heq.
+    
+    destruct B; revgoals.
+    - destruct (decide (m= 0)) as [->|Nneq]; [lia| ]. 
+      iModIntro.
+      subst N.
+
+      iApply sswp_MU_wp; [done| ].
+      iApply (wp_cmpxchg_suc with "[$]"); try done.
+      iIntros "!> Hb". 
+
+      iApply (MU_wand with "[-Hf MU_no]").
+      2: { iSpecialize ("MU_no" with "[] [Hf]").
+           { iPureIntro. lia. }
+           2: { by iFrame. }
+           iSplitL. 
+           { erewrite insert_empty_fmap_helper. by iFrame. }
+           iPureIntro. set_solver. }
+
+      iIntros "[Hf CLOS]".
+
+      iMod (no_update (m - 1) with "[$]") as "[Han Hno]".
+      wp_pures.
+      iModIntro. 
+      iMod ("CLOS" with "[Hb Hay Han]") as "_".
+      { iNext. iFrame. iPureIntro. by intros [=]. }
+      iModIntro.
+
+      rewrite map_union_empty. 
+      simpl in *. wp_load. wp_store. wp_load. wp_pure _.
+      destruct m; [lia| ]. 
+      destruct m. 
+      + rewrite bool_decide_eq_false_2; [| lia]. 
+        iApply wp_atomic.
+
+        iPoseProof "VS" as "-#V".
+        clear Hnever. 
+        iMod "V" as "(%m & %B & ((>%Hnever & >Bb & Hauths) & V))".
+        iDestruct (bi.and_elim_r with "V") as "DEALLOC".
+
+        rewrite if_arg2_comm. iDestruct "Hauths" as "[Hay Han]". 
+        rewrite !if_arg_comm. iMod "Hay". iMod "Han".
+        iDestruct (no_agree with "Hno Han") as %Heq.
+        
+        iAssert (⌜ m = 0 /\ B = true ⌝)%I as %EQ.
+        { iPureIntro. destruct B; [tauto| ]. set_solver. }
+        iModIntro. 
+        
+        iApply wp_pre_step. wp_pure _. 
+        iApply fupd_mask_intro; [done|].
+        iIntros "Hclose'".
+
+        destruct EQ as [-> ->]. 
+        iSpecialize ("DEALLOC" with "[//] [Hf]").
+        { iSplitL.
+          { erewrite insert_empty_fmap_helper. by iFrame. }
+          iPureIntro. rewrite dom_fmap. set_solver. }
+        Unshelve. 2: exact id. 
+ 
+        iApply (pre_step_mono with "[-DEALLOC] [$]").
+        iIntros "[MAP CORR]".
+        iMod ("CORR" with "[Bb Hay Han]").
+        { iNext. iFrame. done. }
+        by iApply "Hk". 
+      + rewrite bool_decide_eq_true_2 //; [| lia].
+        wp_pure _.
+        iApply ("Hg" with "[] [Hf Hno HnN] [$]"); last first.
+        { iFrame "∗#". iSplit; last by iPureIntro; lia.
+          by rewrite Nat2Z.inj_sub; [| lia]. }
+        iPureIntro; lia.
+    - have HM: m> 0 by lia.
+      iModIntro.
+
+      iApply sswp_MU_wp; [done| ].
+      iApply (wp_cmpxchg_fail with "[$]"); try done.
+      iIntros "!> Hb".
+ 
+      iApply (MU_wand with "[-MU_no Hf]").
+      2: { iSpecialize ("MU_no" with "[] [Hf]").
+           { iPureIntro. lia. }
+           2: by iFrame.
+           iSplitL.
+           { erewrite insert_empty_fmap_helper; by iFrame. }
+           iPureIntro. set_solver. }
+
+      iIntros "[Hf CLOS]".
+      wp_pures. iModIntro.
+      iMod ("CLOS" with "[Hb Hay Han]").
+      { iNext. iFrame. done. }
+      iModIntro.
+      rewrite map_union_empty. 
+      simpl. wp_load. wp_pure _. rewrite bool_decide_eq_true_2; last lia.
+      wp_pure _.
+      iApply ("Hg" with "[] [HNo HnN Hf] [$]"); last first.
+      { iFrame "∗#". iPureIntro; lia. }
+      iPureIntro; lia.
+  Qed.  
 
   Lemma no_spec tid b (N: nat) f (Hf: f > 50):
-    {{{ split_inv Ns__split ∗ yesno_inv b ∗ tid ↦M {[ yn_role No := f ]} ∗ ⌜N > 0⌝ ∗ no_at N }}}
+    {{{ split_inv Ns__split ∗ yesno_inv ENV_AM b ∗ tid ↦M {[ yn_role No := f ]} ∗ ⌜N > 0⌝ ∗ no_at N }}}
       no #N #b @ tid
     {{{ RET #(); tid ↦M ∅ }}}.
   Proof using INDEP.
-    iIntros (Φ) "(#SPLIT & #Hinv & Hf & %HN & Hyes) Hk". unfold no.
-    wp_pures. wp_bind (Alloc _).
+    iIntros (Φ) "(#SPLIT & #Hinv & Hf & %HN & Hno) Hk". unfold no.
+    wp_pures.
+    wp_bind (Alloc _).
     iApply (wp_step_fuel with "[Hf]").
     { apply map_non_empty_singleton. }
     { rewrite has_fuels_gt_1; last by solve_fuel_positive.
       rewrite fmap_insert fmap_empty. done. }
     iApply wp_alloc. iNext. iIntros (n) "HnN _ Hf". wp_pures. iModIntro. wp_pures.
-    iApply (no_go_spec with "[-Hk]"); try iFrame.
+    iApply (no_go_spec_vs with "[-Hk]"); try iFrame.
     { lia. }
-    iFrame "SPLIT Hinv". done. 
-  Qed.
+    iSplit; [| done].
+    (* iApply (yes_vs_from_invs with "[$]").  *)
+  Admitted. 
 
 End proof.
 
