fairis/heap_lang/examples/yesno/yesno_model.v
@@ -1,0 +1,137 @@
+From iris.base_logic.lib Require Import invariants.
+From iris.proofmode Require Import tactics.
+From trillium.fairness Require Import fairness action_model utils.
+
+Open Scope nat.
+
+(** * Definition of the model! *)
+
+Inductive YN := Y | No.
+
+#[global] Instance YN_eqdec: EqDecision YN.
+Proof. solve_decision. Qed.
+
+#[global] Instance YN_countable: Countable YN.
+Proof.
+  refine ({|
+             encode yn := match yn with Y => 1 | No => 2 end;
+             decode p := match p with 1 => Some Y | 2 => Some No | _ => None end;
+         |})%positive.
+  intros yn. by destruct yn.
+Qed.
+
+#[global] Instance YN_inhabited: Inhabited YN.
+Proof. exact (populate Y). Qed.
+
+Definition yn_act: Action := coPpick (↑ nroot .@ "yesno"). 
+
+Inductive yntrans: nat*bool -> (Action * option YN) -> nat*bool -> Prop :=
+| yes_trans n: (n > 0)%nat -> yntrans (n, true) (yn_act, Some Y) (n, false) (* < *)
+| yes_fail n: (n > 1)%nat -> yntrans (n, false) (yn_act, Some Y) (n, false) (* ≤ *)
+| no_trans n: yntrans (S n, false) (yn_act, Some No) (n, true) (* < *)
+| no_fail n: (n > 0)%nat → yntrans (n, true) (yn_act, Some No) (n, true) (* ≤ *)
+.
+
+Definition yn_live_roles nb : gset YN :=
+  match nb with
+  | (0, _) => ∅
+  | (1, false) => {[ No ]}
+  | _ => {[ No; Y ]}
+  end.
+
+Definition yn_AM: ActionModel := {| amTrans := yntrans |}.
+
+Instance yn_step_dec: AM_step_dec yn_AM. 
+Proof. 
+  red. intros [n1 b1] a oρ [n2 b2].
+  Local Ltac nostep := right; intros STEP; inversion STEP; try (subst; tauto || lia). 
+  destruct (decide (a = yn_act)) as [-> | ].
+  2: { by nostep. }
+  destruct oρ as [ρ| ]; [| by nostep].
+  destruct (decide (n2 = n1 /\ b1 = true /\ b2 = false /\ ρ = Y /\ 0 < n1)) as [S| ]. 
+  { destruct S as (->&->&->&->&?).
+    left. simpl. by constructor. } 
+  destruct (decide (n2 = n1 /\ b1 = false /\ b2 = false /\ ρ = Y /\ 1 < n1)) as [S| ]. 
+  { destruct S as (->&->&->&->&?).
+    left. simpl. by constructor. } 
+  destruct (decide (n1 = S n2 /\ b1 = false /\ b2 = true /\ ρ = No)) as [S| ]. 
+  { destruct S as (->&->&->&->).
+    left. simpl. by constructor. } 
+  destruct (decide (n2 = n1 /\ b1 = true /\ b2 = true /\ ρ = No /\ 0 < n1)) as [S| ]. 
+  { destruct S as (->&->&->&->&?).
+    left. simpl. by constructor. }
+  by nostep.
+Qed. 
+
+Instance yn_fb: AM_fin_branch' yn_AM.
+Proof.
+  exists (fun '(n, b) => 
+         n' ← [n; (n-1)%nat];
+         w' ← [b; negb b];
+         ℓ ← [Some Y; Some No];
+         mret ((n', w'), yn_act, ℓ)). 
+  intros [??] [??] ?? Htrans.
+  repeat setoid_rewrite elem_of_list_bind.
+  setoid_rewrite elem_of_list_ret.
+  setoid_rewrite (and_comm (exists _, _) _).
+  setoid_rewrite <- utils.ex_and_comm. rewrite utils.ex_prod'.
+  setoid_rewrite (and_comm _ (_ /\ _)).
+  setoid_rewrite <- (and_assoc _ _). 
+  setoid_rewrite (and_comm _ (_ /\ _)).
+  setoid_rewrite <- utils.ex_and_comm. rewrite utils.ex_prod'.
+  eapply utils.ex_det_iff.
+  { intros [[? ?] ?] (?&EQ&?). simpl in EQ.
+    inversion EQ. subst. reflexivity. }
+  simpl.
+  inversion Htrans; subst; simpl; try set_solver.
+  repeat split; try set_solver.
+  rewrite Nat.sub_0_r. set_solver.
+Qed. 
+
+Lemma yn_AM_live_roles (nb: amSt yn_AM) ρ:
+  ρ ∈ AM_live_roles nb <-> ρ ∈ yn_live_roles nb.
+Proof.
+  destruct nb as [n b]. 
+  rewrite -AM_live_roles_spec. simpl.
+  destruct n as [| [| ]], b; simpl.
+  - split; [| done]. intros (?&?&STEP). inversion STEP; lia.
+  - split; [| done]. intros (?&?&STEP). inversion STEP; lia.
+  - split.
+    + intros (?&?&STEP). inversion STEP; set_solver.
+    + rewrite elem_of_union !elem_of_singleton. intros [-> | ->].
+      all: do 2 eexists; constructor; lia.  
+  - rewrite !elem_of_singleton. 
+    split.
+    + intros (?&?&STEP). inversion STEP; try lia || done.
+    + intros ->. do 2 eexists. constructor.
+  - split.
+    + intros (?&?&STEP). inversion STEP; set_solver.
+    + rewrite elem_of_union !elem_of_singleton. intros [-> | ->].
+      all: do 2 eexists; constructor; lia.  
+  - split.
+    + intros (?&?&STEP). inversion STEP; set_solver.
+    + rewrite elem_of_union !elem_of_singleton. intros [-> | ->].
+      all: do 2 eexists; constructor; lia.  
+Qed.
+
+Lemma yn_acts: forall a, is_action_of yn_AM a <-> a = yn_act.
+Proof. 
+  intros. rewrite /is_action_of. split.
+  - intros (?&?&?&STEP). inversion STEP; eauto.
+  - intros ->.
+    do 3 eexists. econstructor. eauto.
+Qed. 
+
+Lemma yn_AM_live_roles' (st: amSt yn_AM):
+  AM_live_roles st = yn_live_roles st.
+Proof. 
+  apply set_eq. intros. rewrite -yn_AM_live_roles. done.
+Qed. 
+
+Instance yn_AM_act_dec: forall a, Decision (is_action_of yn_AM a).
+Proof.
+  intros. eapply Decision_iff_impl; [symmetry; apply yn_acts| ].
+  apply _.
+Qed. 
+
+
